git/fgdorais/GMLAlgebra/lakefile.lean
@@ -2,9 +2,10 @@ import Lake
 open Lake DSL
 
 package GMLAlgebra {
-  defaultFacet := PackageFacet.oleans
-  dependencies := #[{
-    name := `GMLInit
-    src := Source.git "https://github.com/fgdorais/GMLInit.git" "384f93fb25b8d6e81dcf2abc396d9472568d88af"
-  }]
+  moreLeanArgs := #["-Dlinter.unusedVariables=false"]
 }
+
+@[defaultTarget]
+lean_lib GMLAlgebra {}
+
+require GMLInit from git "https://github.com/fgdorais/GMLInit.git"@"4e5230249bd8788a7880d11d05436ee4b70b6c33"
