git/leanprover/lake/Lake/CLI/Build.lean
@@ -39,7 +39,7 @@ def resolveModuleTarget (ws : Workspace) (mod : Module) (facet : String) : Excep
   else if facet == "dynlib" then
     return mod.facetTarget dynlibFacet
   else if let some config := ws.findModuleFacetConfig? facet then
-    return mod.facetTarget config.facet
+    return mod.facetTarget config.name
   else
     throw <| CliError.unknownFacet "module" facet
 
@@ -60,7 +60,9 @@ def resolveExeTarget (exe : LeanExe) (facet : String) : Except CliError OpaqueTa
     throw <| CliError.unknownFacet "executable" facet
 
 def resolveTargetInPackage (ws : Workspace) (pkg : Package) (target : Name) (facet : String) : Except CliError OpaqueTarget :=
-  if let some exe := pkg.findLeanExe? target then
+  if let some target := pkg.findTargetConfig? target then
+    return pkg.facet target.name |>.target
+  else if let some exe := pkg.findLeanExe? target then
     resolveExeTarget exe facet
   else if let some lib := pkg.findExternLib? target then
     if facet.isEmpty then
@@ -92,11 +94,15 @@ def resolvePackageTarget (ws : Workspace) (pkg : Package) (facet : String) : Exc
     return pkg.sharedLibTarget.withoutInfo
   else if facet == "leanLib" || facet == "oleans" then
     return pkg.leanLibTarget.withoutInfo
+  else if let some config := ws.findPackageFacetConfig? facet then
+    return pkg.facet config.name |>.target
   else
     throw <| CliError.unknownFacet "package" facet
 
 def resolveTargetInWorkspace (ws : Workspace) (spec : String) (facet : String) : Except CliError OpaqueTarget :=
-  if let some exe := ws.findLeanExe? spec.toName then
+  if let some (pkg, target) := ws.findTargetConfig? spec then
+    return pkg.facet target.name |>.target
+  else if let some exe := ws.findLeanExe? spec.toName then
     resolveExeTarget exe facet
   else if let some lib := ws.findExternLib? spec.toName then
     if facet.isEmpty then
