git/leanprover/lake/examples/targets/lakefile.lean
@@ -15,3 +15,16 @@ lean_exe b
 
 @[defaultTarget]
 lean_exe c
+
+@[defaultTarget]
+target meow : PUnit := fun pkg => do
+  IO.FS.writeFile (pkg.buildDir / "meow.txt") "Meow!"
+  return ActiveTarget.nil
+
+target bark : PUnit := fun _ => do
+  logInfo "Bark!"
+  return ActiveTarget.nil
+
+package_facet print_name : PUnit := fun pkg => do
+  IO.println pkg.name
+  return ActiveTarget.nil
